src/dvspec/dafny/att_spec_proofs/proofs_ind_inv.dfy
@@ -7,9 +7,11 @@ include "../att_spec_proofs/inv.dfy"
 include "../att_spec_proofs/assump.dfy"
 include "../att_spec_proofs/fnc_inv.dfy"
 include "../att_spec_proofs/helper_sets_lemmas.dfy"
+include "../att_spec_proofs/proofs_intermediate_steps.dfy"
 include "../att_spec_proofs/dvn_next_invs_1_7.dfy"
 include "../att_spec_proofs/dvn_next_invs_8_18.dfy"
-include "../att_spec_proofs/proofs_intermediate_steps.dfy"
+include "../att_spec_proofs/dvn_next_invs_19.dfy"
+
 
 module Proofs_DVN_Ind_Inv
 {
@@ -25,12 +27,14 @@ module Proofs_DVN_Ind_Inv
     import opened Helper_Sets_Lemmas
     import opened DVN_Next_Invs_1_7
     import opened DVN_Next_Invs_8_18
+    import opened DVN_Next_Invs_19
     import opened Proofs_Intermediate_Steps
 
     predicate ind_inv(dvn: DVState)       
     {
         && invs_1_7(dvn)
         && invs_8_18(dvn)
+        && invs_19(dvn)
     }
 
     predicate invs_1_7(dvn: DVState)       
@@ -55,10 +59,30 @@ module Proofs_DVN_Ind_Inv
         &&  inv18(dvn)  
     }
 
+    predicate invs_19(dvn: DVState)       
+    {        
+        &&  inv19(dvn)           
+        &&  inv21(dvn) 
+        &&  inv22(dvn)      
+        &&  inv23(dvn)  
+        &&  inv25(dvn)          
+        &&  inv26(dvn)  
+    }
+
     lemma lemma_ind_inv_dvn_init(dvn: DVState)       
     requires DV.Init(dvn, {})    
     ensures ind_inv(dvn)
     {}  
+
+    lemma lemma_ind_inv_dvn_next_ind_inv(dvn: DVState, dvn': DVState)       
+    requires exists e: DV.Event :: DV.NextEvent(dvn, e, dvn')
+    requires ind_inv(dvn)
+    ensures ind_inv(dvn')
+    {
+        lemma_ind_inv_dvn_next_invs_1_7(dvn, dvn');
+        lemma_ind_inv_dvn_next_invs_8_18(dvn, dvn');
+        lemma_ind_inv_dvn_next_invs_19(dvn, dvn');
+    }
 
     lemma lemma_ind_inv_dvn_next_invs_1_7(dvn: DVState, dvn': DVState)       
     requires exists e: DV.Event :: DV.NextEvent(dvn, e, dvn')
@@ -95,18 +119,37 @@ module Proofs_DVN_Ind_Inv
         lemma_inv18_dvn_next(dvn, e, dvn');
     }
 
+    lemma lemma_ind_inv_dvn_next_invs_19(dvn: DVState, dvn': DVState)       
+    requires exists e: DV.Event :: DV.NextEvent(dvn, e, dvn')
+    requires ind_inv(dvn)
+    ensures invs_19(dvn')        
+    {
+        var e: DV.Event :| DV.NextEvent(dvn, e, dvn');
+        lemma_inv19_dvn_next(dvn, e, dvn');
+        lemma_inv20_dvn_next(dvn, e, dvn');
+        lemma_inv21_dvn_next(dvn, e, dvn');        
+        lemma_inv22_dvn_next(dvn, e, dvn');                
+        lemma_inv23_dvn_next(dvn, e, dvn');                
+        lemma_inv25_dvn_next(dvn, e, dvn');    
+        lemma_inv26_dvn_next(dvn, e, dvn');    
+    }
+
     lemma lemma_ind_inv_implies_other_invs(dvn: DVState)
     requires ind_inv(dvn)
     ensures inv11(dvn)
     ensures inv12(dvn)
     ensures inv14(dvn)
     ensures inv15(dvn)
+    ensures inv24(dvn)
     ensures inv53(dvn)    
-    {
-        lemma_inv2_inv53(dvn);
+    ensures inv51(dvn)    
+    {    
+        lemma_inv53_ind_inv(dvn);
         lemma_inv15_ind_inv(dvn);
         lemma_inv14_ind_inv(dvn);
         lemma_inv12_ind_inv(dvn);
         lemma_inv11_ind_inv(dvn);
+        lemma_inv24_ind_inv(dvn);
+        lemma_inv51_ind_inv(dvn);
     }
 }
