src/dvspec/dafny/att_spec_proofs/fnc_inv.dfy
@@ -5,6 +5,7 @@ include "../specification/network.dfy"
 include "../specification/dvn.dfy"
 include "../att_spec_proofs/inv.dfy"
 include "../att_spec_proofs/assump.dfy"
+include "../att_spec_proofs/helper_sets_lemmas.dfy"
 
 
 module Fnc_Inv
@@ -17,7 +18,9 @@ module Fnc_Inv
     import opened DV
     import opened Att_Inv_With_Empty_Initial_Attestation_Slashing_DB
     import opened Att_Assumptions
+    import opened Helper_Sets_Lemmas
 
+    
     
     lemma lemma_inv4_f_serve_attestation_duty(
         dvc: DVCNodeState,
@@ -2530,4 +2533,563 @@ module Fnc_Inv
         assert process' == res.state;
         assert inv23_body(process');
     } 
+
+    lemma lemma_inv25_add_block_to_bn(
+        s: DVCNodeState,
+        block: BeaconBlock,
+        s': DVCNodeState 
+    )
+    requires add_block_to_bn.requires(s, block)
+    requires s' == add_block_to_bn(s, block)    
+    requires inv25_body(s)
+    ensures inv25_body(s')
+    { }
+
+    lemma lemma_inv25_f_listen_for_attestation_shares(
+        process: DVCNodeState,
+        attestation_share: AttestationShare,
+        process': DVCNodeState
+    )
+    requires f_listen_for_attestation_shares.requires(process, attestation_share)
+    requires process' == f_listen_for_attestation_shares(process, attestation_share).state        
+    requires inv25_body(process)
+    ensures inv25_body(process')
+    { }
+
+    lemma lemma_inv25_f_start_next_duty(process: DVCNodeState, attestation_duty: AttestationDuty, process': DVCNodeState)
+    requires f_start_next_duty.requires(process, attestation_duty)
+    requires process' == f_start_next_duty(process, attestation_duty).state   
+    requires attestation_duty in process.all_rcvd_duties
+    requires inv25_body(process)
+    ensures inv25_body(process')
+    { } 
+
+    lemma lemma_inv25_f_resend_attestation_share(
+        process: DVCNodeState,
+        process': DVCNodeState)
+    requires f_resend_attestation_share.requires(process)
+    requires process' == f_resend_attestation_share(process).state        
+    requires inv25_body(process)
+    ensures inv25_body(process')
+    { } 
+
+    lemma lemma_inv25_f_check_for_next_queued_duty(
+        process: DVCNodeState,
+        process': DVCNodeState
+    )
+    requires f_check_for_next_queued_duty.requires(process)
+    requires process' == f_check_for_next_queued_duty(process).state    
+    requires inv5_body(process)
+    requires inv25_body(process)
+    ensures inv25_body(process')
+    decreases process.attestation_duties_queue
+    {
+        if  && process.attestation_duties_queue != [] 
+            && (
+                || process.attestation_duties_queue[0].slot in process.future_att_consensus_instances_already_decided
+                || !process.current_attestation_duty.isPresent()
+            )    
+        {            
+                if process.attestation_duties_queue[0].slot in process.future_att_consensus_instances_already_decided.Keys 
+                {
+                    var queue_head := process.attestation_duties_queue[0];
+                    var new_attestation_slashing_db := f_update_attestation_slashing_db(process.attestation_slashing_db, process.future_att_consensus_instances_already_decided[queue_head.slot]);
+                    var process_mod := process.(
+                        attestation_duties_queue := process.attestation_duties_queue[1..],
+                        future_att_consensus_instances_already_decided := process.future_att_consensus_instances_already_decided - {queue_head.slot},
+                        attestation_slashing_db := new_attestation_slashing_db,
+                        attestation_consensus_engine_state := updateConsensusInstanceValidityCheck(
+                            process.attestation_consensus_engine_state,
+                            new_attestation_slashing_db
+                        )                        
+                    );
+                    assert inv5_body(process_mod);
+                    lemma_inv25_f_check_for_next_queued_duty(process_mod, process');
+                }
+                else
+                { 
+                    var process_mod := process.(
+                        attestation_duties_queue := process.attestation_duties_queue[1..]
+                    );     
+                    assert inv25_body(process_mod);
+
+                    lemma_inv25_f_start_next_duty(process_mod, process.attestation_duties_queue[0], process');
+                }
+        }
+        else
+        { 
+            assert process'.all_rcvd_duties == process.all_rcvd_duties;
+        }
+    }
+
+    lemma lemma_inv25_f_att_consensus_decided(
+        process: DVCNodeState,
+        id: Slot,
+        decided_attestation_data: AttestationData, 
+        process': DVCNodeState
+    )
+    requires f_att_consensus_decided.requires(process, id, decided_attestation_data)
+    requires process' == f_att_consensus_decided(process, id, decided_attestation_data).state         
+    requires inv5_body(process)
+    requires inv25_body(process)
+    ensures inv25_body(process')
+    {
+        
+        var local_current_attestation_duty := process.current_attestation_duty.safe_get();
+        var attestation_slashing_db := f_update_attestation_slashing_db(process.attestation_slashing_db, decided_attestation_data);
+
+        var fork_version := bn_get_fork_version(compute_start_slot_at_epoch(decided_attestation_data.target.epoch));
+        var attestation_signing_root := compute_attestation_signing_root(decided_attestation_data, fork_version);
+        var attestation_signature_share := rs_sign_attestation(decided_attestation_data, fork_version, attestation_signing_root, process.rs);
+        var attestation_with_signature_share := AttestationShare(
+                aggregation_bits := get_aggregation_bits(local_current_attestation_duty.validator_index),
+                data := decided_attestation_data, 
+                signature := attestation_signature_share
+            ); 
+
+        var process := 
+            process.(
+                current_attestation_duty := None,
+                attestation_shares_to_broadcast := process.attestation_shares_to_broadcast[local_current_attestation_duty.slot := attestation_with_signature_share],
+                attestation_slashing_db := attestation_slashing_db,
+                attestation_consensus_engine_state := updateConsensusInstanceValidityCheck(
+                    process.attestation_consensus_engine_state,
+                    attestation_slashing_db
+                )
+            );
+
+        assert inv5_body(process);
+        assert inv25_body(process);
+
+        var ret_dvc := f_check_for_next_queued_duty(process).state;
+        lemma_inv5_f_check_for_next_queued_duty(process, ret_dvc);
+        assert inv5_body(ret_dvc);
+        
+        lemma_inv25_f_check_for_next_queued_duty(process, ret_dvc);
+        assert inv25_body(ret_dvc);
+
+        assert process' == ret_dvc;        
+    }
+
+    lemma lemma_inv25_f_serve_attestation_duty(
+        process: DVCNodeState,
+        attestation_duty: AttestationDuty,
+        process': DVCNodeState
+    )  
+    requires f_serve_attestation_duty.requires(process, attestation_duty)
+    requires process' == f_serve_attestation_duty(process, attestation_duty).state
+    requires inv5_body(process)
+    requires inv25_body(process)
+    ensures inv25_body(process')
+    {
+        var process_mod := process.(
+                attestation_duties_queue := process.attestation_duties_queue + [attestation_duty],
+                all_rcvd_duties := process.all_rcvd_duties + {attestation_duty}
+            );        
+
+        assert inv5_body(process_mod);
+        assert inv25_body(process_mod);
+        
+        lemma_inv25_f_check_for_next_queued_duty(process_mod, process');        
+    }
+
+    lemma lemma_inv25_f_listen_for_new_imported_blocks(
+        process: DVCNodeState,
+        block: BeaconBlock,
+        process': DVCNodeState
+    )
+    requires f_listen_for_new_imported_blocks.requires(process, block)
+    requires process' == f_listen_for_new_imported_blocks(process, block).state        
+    requires inv5_body(process)
+    requires inv25_body(process)
+    ensures inv25_body(process')
+    {
+        var new_consensus_instances_already_decided := f_listen_for_new_imported_blocks_helper_1(process, block);
+
+        var att_consensus_instances_already_decided := process.future_att_consensus_instances_already_decided + new_consensus_instances_already_decided;
+
+        var future_att_consensus_instances_already_decided := 
+            f_listen_for_new_imported_blocks_helper_2(process, att_consensus_instances_already_decided);
+
+        var process :=
+                process.(
+                    future_att_consensus_instances_already_decided := future_att_consensus_instances_already_decided,
+                    attestation_consensus_engine_state := stopConsensusInstances(
+                                    process.attestation_consensus_engine_state,
+                                    att_consensus_instances_already_decided.Keys
+                    ),
+                    attestation_shares_to_broadcast := process.attestation_shares_to_broadcast - att_consensus_instances_already_decided.Keys,
+                    rcvd_attestation_shares := process.rcvd_attestation_shares - att_consensus_instances_already_decided.Keys                    
+                );    
+        
+        assert inv5_body(process);
+        assert inv25_body(process);
+
+        if process.current_attestation_duty.isPresent() && process.current_attestation_duty.safe_get().slot in att_consensus_instances_already_decided
+        {
+            var decided_attestation_data := att_consensus_instances_already_decided[process.current_attestation_duty.safe_get().slot];
+            var new_attestation_slashing_db := f_update_attestation_slashing_db(process.attestation_slashing_db, decided_attestation_data);
+            var process := process.(
+                current_attestation_duty := None,
+                attestation_slashing_db := new_attestation_slashing_db,
+                attestation_consensus_engine_state := updateConsensusInstanceValidityCheck(
+                    process.attestation_consensus_engine_state,
+                    new_attestation_slashing_db
+                )                
+            );
+            
+            assert inv5_body(process);
+            assert inv25_body(process);
+
+            lemma_inv25_f_check_for_next_queued_duty(process, process');
+        }
+        else
+        {               
+            assert inv25_body(process);
+        }
+    } 
+
+    lemma lemma_inv26_add_block_to_bn(
+        s: DVCNodeState,
+        block: BeaconBlock,
+        s': DVCNodeState 
+    )
+    requires add_block_to_bn.requires(s, block)
+    requires s' == add_block_to_bn(s, block)    
+    requires inv26_body(s)
+    ensures inv26_body(s')
+    { }
+
+    lemma lemma_inv26_f_listen_for_attestation_shares(
+        process: DVCNodeState,
+        attestation_share: AttestationShare,
+        process': DVCNodeState
+    )
+    requires f_listen_for_attestation_shares.requires(process, attestation_share)
+    requires process' == f_listen_for_attestation_shares(process, attestation_share).state        
+    requires inv26_body(process)
+    ensures inv26_body(process')
+    { }
+
+    lemma lemma_inv26_f_start_next_duty(process: DVCNodeState, attestation_duty: AttestationDuty, process': DVCNodeState)
+    requires f_start_next_duty.requires(process, attestation_duty)
+    requires process' == f_start_next_duty(process, attestation_duty).state   
+    requires attestation_duty in process.all_rcvd_duties
+    requires inv26_body(process)
+    ensures inv26_body(process')
+    { } 
+
+    lemma lemma_inv26_f_resend_attestation_share(
+        process: DVCNodeState,
+        process': DVCNodeState)
+    requires f_resend_attestation_share.requires(process)
+    requires process' == f_resend_attestation_share(process).state        
+    requires inv26_body(process)
+    ensures inv26_body(process')
+    { } 
+
+    lemma lemma_updateConsensusInstanceValidityCheckHelper(
+        m: map<Slot, AttestationConsensusValidityCheckState>,
+        new_attestation_slashing_db: set<SlashingDBAttestation>,
+        m': map<Slot, AttestationConsensusValidityCheckState>
+    )    
+    requires m' == updateConsensusInstanceValidityCheckHelper(m, new_attestation_slashing_db)
+    ensures m.Keys == m'.Keys
+    ensures forall slot |
+                && slot in m'.Keys 
+                ::
+                var acvc := m'[slot];
+                && acvc.validityPredicate == ((ad: AttestationData) => consensus_is_valid_attestation_data(new_attestation_slashing_db, ad, acvc.attestation_duty));
+  
+    {
+        forall k | k in  m 
+        ensures k in m'
+        {
+            lemmaMapKeysHasOneEntryInItems(m, k);
+            assert k in m';
+        }
+
+        assert m.Keys == m'.Keys;
+
+        assert forall slot |
+                && slot in m'.Keys 
+                ::
+                var acvc := m'[slot];
+                && acvc.validityPredicate == (ad: AttestationData) => consensus_is_valid_attestation_data(new_attestation_slashing_db, ad, acvc.attestation_duty);
+
+    }  
+
+    lemma lemma_inv26_f_check_for_next_queued_duty(
+        process: DVCNodeState,
+        process': DVCNodeState
+    )
+    requires f_check_for_next_queued_duty.requires(process)
+    requires process' == f_check_for_next_queued_duty(process).state    
+    requires inv5_body(process)
+    requires inv25_body(process)
+    requires inv26_body(process)
+    ensures inv26_body(process')
+    decreases process.attestation_duties_queue
+    {
+        if  && process.attestation_duties_queue != [] 
+            && (
+                || process.attestation_duties_queue[0].slot in process.future_att_consensus_instances_already_decided
+                || !process.current_attestation_duty.isPresent()
+            )    
+        {            
+                if process.attestation_duties_queue[0].slot in process.future_att_consensus_instances_already_decided.Keys 
+                {
+                    var queue_head := process.attestation_duties_queue[0];
+                    var new_attestation_slashing_db := f_update_attestation_slashing_db(process.attestation_slashing_db, process.future_att_consensus_instances_already_decided[queue_head.slot]);
+                    var process_mod := process.(
+                        attestation_duties_queue := process.attestation_duties_queue[1..],
+                        future_att_consensus_instances_already_decided := process.future_att_consensus_instances_already_decided - {queue_head.slot},
+                        attestation_slashing_db := new_attestation_slashing_db,
+                        attestation_consensus_engine_state := updateConsensusInstanceValidityCheck(
+                            process.attestation_consensus_engine_state,
+                            new_attestation_slashing_db
+                        )                        
+                    );
+
+                    lemma_updateConsensusInstanceValidityCheck(
+                                process.attestation_consensus_engine_state,
+                                new_attestation_slashing_db,
+                                process_mod.attestation_consensus_engine_state 
+                                );
+
+                    assert process_mod.attestation_consensus_engine_state.att_slashing_db_hist.Keys
+                                == process.attestation_consensus_engine_state.att_slashing_db_hist.Keys 
+                                        + process.attestation_consensus_engine_state.attestation_consensus_active_instances.Keys;
+
+                    assert inv25_body(process_mod);
+
+                    assert inv5_body(process_mod);
+                    assert inv26_body(process_mod);
+                    lemma_inv26_f_check_for_next_queued_duty(process_mod, process');
+                }
+                else
+                { 
+                    var process_mod := process.(
+                        attestation_duties_queue := process.attestation_duties_queue[1..]
+                    );     
+                    assert inv5_body(process_mod);
+                    assert inv26_body(process_mod);
+                    lemma_inv26_f_start_next_duty(process_mod, process.attestation_duties_queue[0], process');
+                }
+        }
+        else
+        { 
+            assert process'.all_rcvd_duties == process.all_rcvd_duties;
+        }
+    }
+
+    lemma lemma_updateConsensusInstanceValidityCheck(
+        s: ConsensusEngineState,
+        new_attestation_slashing_db: set<SlashingDBAttestation>,
+        r: ConsensusEngineState
+    )
+    requires r == updateConsensusInstanceValidityCheck(s, new_attestation_slashing_db)        
+    ensures r.att_slashing_db_hist.Keys
+                == s.att_slashing_db_hist.Keys + s.attestation_consensus_active_instances.Keys
+    {
+        var new_attestation_consensus_active_instances := updateConsensusInstanceValidityCheckHelper(
+                    s.attestation_consensus_active_instances,
+                    new_attestation_slashing_db
+                );
+
+        lemma_updateConsensusInstanceValidityCheckHelper(
+                s.attestation_consensus_active_instances,
+                new_attestation_slashing_db,
+                new_attestation_consensus_active_instances);
+
+        assert new_attestation_consensus_active_instances.Keys == s.attestation_consensus_active_instances.Keys;
+
+        var new_att_slashing_db_hist := updateAttSlashingDBHist(
+                                            s.att_slashing_db_hist,
+                                            new_attestation_consensus_active_instances,
+                                            new_attestation_slashing_db
+                                        );
+
+        assert new_att_slashing_db_hist.Keys 
+                    == s.att_slashing_db_hist.Keys + new_attestation_consensus_active_instances.Keys;
+
+        var t := s.(attestation_consensus_active_instances := new_attestation_consensus_active_instances,
+                    att_slashing_db_hist := new_att_slashing_db_hist
+                   );
+
+        assert r.att_slashing_db_hist.Keys == t.att_slashing_db_hist.Keys;
+
+        calc 
+        {
+            r.att_slashing_db_hist.Keys;
+            ==
+            t.att_slashing_db_hist.Keys;
+            ==
+            new_att_slashing_db_hist.Keys;
+            == 
+            s.att_slashing_db_hist.Keys + new_attestation_consensus_active_instances.Keys;
+            ==
+            s.att_slashing_db_hist.Keys + s.attestation_consensus_active_instances.Keys;
+        }
+    }
+
+    lemma lemma_inv26_f_att_consensus_decided(
+        process: DVCNodeState,
+        id: Slot,
+        decided_attestation_data: AttestationData, 
+        process': DVCNodeState
+    )
+    requires f_att_consensus_decided.requires(process, id, decided_attestation_data)
+    requires process' == f_att_consensus_decided(process, id, decided_attestation_data).state         
+    requires inv5_body(process)
+    requires inv25_body(process)
+    requires inv26_body(process)
+    ensures inv26_body(process')
+    {
+        
+        var local_current_attestation_duty := process.current_attestation_duty.safe_get();
+        var attestation_slashing_db := f_update_attestation_slashing_db(process.attestation_slashing_db, decided_attestation_data);
+
+        var fork_version := bn_get_fork_version(compute_start_slot_at_epoch(decided_attestation_data.target.epoch));
+        var attestation_signing_root := compute_attestation_signing_root(decided_attestation_data, fork_version);
+        var attestation_signature_share := rs_sign_attestation(decided_attestation_data, fork_version, attestation_signing_root, process.rs);
+        var attestation_with_signature_share := AttestationShare(
+                aggregation_bits := get_aggregation_bits(local_current_attestation_duty.validator_index),
+                data := decided_attestation_data, 
+                signature := attestation_signature_share
+            ); 
+
+        var new_attestation_consensus_engine_state := updateConsensusInstanceValidityCheck(
+                                                            process.attestation_consensus_engine_state,
+                                                            attestation_slashing_db
+                                                      );
+
+        var process_mod := 
+            process.(
+                current_attestation_duty := None,
+                attestation_shares_to_broadcast := process.attestation_shares_to_broadcast[local_current_attestation_duty.slot := attestation_with_signature_share],
+                attestation_slashing_db := attestation_slashing_db,
+                attestation_consensus_engine_state := new_attestation_consensus_engine_state
+            );
+    
+        lemma_updateConsensusInstanceValidityCheck(
+                                process.attestation_consensus_engine_state,
+                                attestation_slashing_db,
+                                process_mod.attestation_consensus_engine_state 
+                                );
+
+        assert process_mod.attestation_consensus_engine_state.att_slashing_db_hist.Keys
+                    == process.attestation_consensus_engine_state.att_slashing_db_hist.Keys 
+                            + process.attestation_consensus_engine_state.attestation_consensus_active_instances.Keys;
+
+
+        assert inv5_body(process_mod);
+        assert inv25_body(process_mod);
+
+        assert inv26_body(process_mod);
+
+        var ret_dvc := f_check_for_next_queued_duty(process_mod).state;
+        lemma_inv5_f_check_for_next_queued_duty(process_mod, ret_dvc);
+        assert inv5_body(ret_dvc);
+        
+        lemma_inv26_f_check_for_next_queued_duty(process_mod, ret_dvc);
+        assert inv26_body(ret_dvc);
+
+        assert process' == ret_dvc;        
+    }
+
+    lemma lemma_inv26_f_serve_attestation_duty(
+        process: DVCNodeState,
+        attestation_duty: AttestationDuty,
+        process': DVCNodeState
+    )  
+    requires f_serve_attestation_duty.requires(process, attestation_duty)
+    requires process' == f_serve_attestation_duty(process, attestation_duty).state
+    requires inv5_body(process)
+    requires inv25_body(process)
+    requires inv26_body(process)
+    ensures inv26_body(process')
+    {
+        var process_mod := process.(
+                attestation_duties_queue := process.attestation_duties_queue + [attestation_duty],
+                all_rcvd_duties := process.all_rcvd_duties + {attestation_duty}
+            );        
+
+        assert inv5_body(process_mod);
+        assert inv25_body(process_mod);
+        assert inv26_body(process_mod);
+        
+        lemma_inv26_f_check_for_next_queued_duty(process_mod, process');        
+    }
+
+    lemma lemma_inv26_f_listen_for_new_imported_blocks(
+        process: DVCNodeState,
+        block: BeaconBlock,
+        process': DVCNodeState
+    )
+    requires f_listen_for_new_imported_blocks.requires(process, block)
+    requires process' == f_listen_for_new_imported_blocks(process, block).state        
+    requires inv5_body(process)
+    requires inv25_body(process)
+    requires inv26_body(process)
+    ensures inv26_body(process')
+    {
+        var new_consensus_instances_already_decided := f_listen_for_new_imported_blocks_helper_1(process, block);
+
+        var att_consensus_instances_already_decided := process.future_att_consensus_instances_already_decided + new_consensus_instances_already_decided;
+
+        var future_att_consensus_instances_already_decided := 
+            f_listen_for_new_imported_blocks_helper_2(process, att_consensus_instances_already_decided);
+
+        var process :=
+                process.(
+                    future_att_consensus_instances_already_decided := future_att_consensus_instances_already_decided,
+                    attestation_consensus_engine_state := stopConsensusInstances(
+                                    process.attestation_consensus_engine_state,
+                                    att_consensus_instances_already_decided.Keys
+                    ),
+                    attestation_shares_to_broadcast := process.attestation_shares_to_broadcast - att_consensus_instances_already_decided.Keys,
+                    rcvd_attestation_shares := process.rcvd_attestation_shares - att_consensus_instances_already_decided.Keys                    
+                );    
+        
+        assert inv5_body(process);
+        assert inv25_body(process);
+        assert inv26_body(process);
+
+        if process.current_attestation_duty.isPresent() && process.current_attestation_duty.safe_get().slot in att_consensus_instances_already_decided
+        {
+            var decided_attestation_data := att_consensus_instances_already_decided[process.current_attestation_duty.safe_get().slot];
+            var new_attestation_slashing_db := f_update_attestation_slashing_db(process.attestation_slashing_db, decided_attestation_data);
+            var new_attestation_consensus_engine_state := updateConsensusInstanceValidityCheck(
+                                                            process.attestation_consensus_engine_state,
+                                                            new_attestation_slashing_db
+                                                          );  
+            var process_mod := process.(
+                current_attestation_duty := None,
+                attestation_slashing_db := new_attestation_slashing_db,
+                attestation_consensus_engine_state := new_attestation_consensus_engine_state
+            );
+
+            lemma_updateConsensusInstanceValidityCheck(
+                                process.attestation_consensus_engine_state,
+                                new_attestation_slashing_db,
+                                process_mod.attestation_consensus_engine_state 
+                                );
+
+            assert process_mod.attestation_consensus_engine_state.att_slashing_db_hist.Keys
+                    == process.attestation_consensus_engine_state.att_slashing_db_hist.Keys 
+                            + process.attestation_consensus_engine_state.attestation_consensus_active_instances.Keys;
+
+            
+            assert inv5_body(process_mod);
+            assert inv25_body(process_mod);
+            assert inv26_body(process_mod);
+
+            lemma_inv26_f_check_for_next_queued_duty(process_mod, process');
+        }
+        else
+        {               
+            assert inv26_body(process);
+        }
+    }  
 }
