src/dvspec/dafny/att_spec_proofs/incomplete_proofs.dfy
@@ -6,9 +6,10 @@ include "../specification/dvn.dfy"
 include "../att_spec_proofs/inv.dfy"
 include "../att_spec_proofs/assump.dfy"
 include "../att_spec_proofs/fnc_inv.dfy"
+include "../att_spec_proofs/helper_sets_lemmas.dfy"
 include "../att_spec_proofs/dvn_next_invs_1_7.dfy"
 include "../att_spec_proofs/dvn_next_invs_8_18.dfy"
-include "../att_spec_proofs/helper_sets_lemmas.dfy"
+include "../att_spec_proofs/dvn_next_invs_19.dfy"
 
 
 module Incomplete_Proofs 
@@ -23,20 +24,19 @@ module Incomplete_Proofs
     import opened Helper_Sets_Lemmas
     import opened DVN_Next_Invs_1_7
     import opened DVN_Next_Invs_8_18
+    import opened DVN_Next_Invs_19
     import opened Fnc_Inv    
-
-    lemma {:axiom} axiom_inv23(dvn: DVState)    
-    ensures inv23(dvn)
-
     
     
 
+    lemma {:axiom} axiom_inv26(dvn: DVState)    
+    ensures inv26(dvn)
+
+    
     
     
 
     
 
-
-
-    
+      
 }
